string_project/str_recurse_boogie_modification_1_preexe_RES.bpl
@@ -1,29 +1,29 @@
-<no file>(1498,4): Error: This assertion might not hold.
+<no file>(1821,4): Error: This assertion might not hold.
 Execution trace:
-    (1609,3): anon0
+    (1981,3): anon0
 Augmented execution trace:
-Impl | Impl$$M.__default.foo | 11 | 6
-Types | int | int
+Impl | Impl$$M.__default.replaceRecursive | T@U!val!74 | T@U!val!73 | T@U!val!75
+Types | Seq Box | Seq Box | Seq Box
 
 *** MODEL
-#_System._tuple#0._#Make0 -> T@U!val!63
-##_System._tuple#0._#Make0 -> T@U!val!40
-##_System._tuple#2._#Make2 -> T@U!val!37
+#_System._tuple#0._#Make0 -> T@U!val!69
+##_System._tuple#0._#Make0 -> T@U!val!43
+##_System._tuple#2._#Make2 -> T@U!val!40
 $_Frame -> 
-$_Frame@0 -> T@U!val!66
+$_Frame@0 -> T@U!val!83
 $_reverifyPost -> 
 $$Language$Dafny -> true
-$FunctionContextHeight -> 0
-$Heap -> T@U!val!65
-$OneHeap -> T@U!val!58
+$FunctionContextHeight -> 2
+$Heap -> T@U!val!72
+$LZ -> T@U!val!71
+$OneHeap -> T@U!val!64
+$rhs##1_0 -> T@U!val!78
+$rhs##2_0 -> T@U!val!81
 $Tick -> 
-a#0 -> 11
 alloc -> T@U!val!22
 allocName -> T@U!val!23
-b#0 -> 6
 boolType -> T@T!val!2
 BoxType -> T@T!val!13
-c#0 -> 
 charType -> T@T!val!14
 class._System.array? -> T@U!val!28
 class._System.bool -> T@U!val!18
@@ -32,22 +32,35 @@ class._System.multiset -> T@U!val!21
 class._System.object? -> T@U!val!25
 class._System.seq -> T@U!val!20
 class._System.set -> T@U!val!19
-class._System.Tuple0 -> T@U!val!42
-class._System.Tuple2 -> T@U!val!39
-class.M.__default -> T@U!val!43
+class._System.Tuple0 -> T@U!val!45
+class._System.Tuple2 -> T@U!val!42
+class.M.__default -> T@U!val!46
 ClassNameType -> T@T!val!8
 DatatypeTypeType -> T@T!val!17
-defass#c#0 -> 
+defass#newString#0 -> false
 DtCtorIdType -> T@T!val!11
+first#2_0 -> T@U!val!79
 HandleTypeType -> T@T!val!20
+inner#2_0 -> T@U!val!80
 intType -> T@T!val!0
 LayerTypeType -> T@T!val!18
 MapType1Type -> T@T!val!15
 NameFamilyType -> T@T!val!10
-null -> T@U!val!60
+newString#0 -> T@U!val!76
+null -> T@U!val!66
+other##1_0 -> 
+other##2_0 -> 
+other#0@@5 -> T@U!val!75
+pattern##1_0 -> 
+pattern##2_0 -> 
+pattern#0@@5 -> T@U!val!73
+prefixedInner#1_0 -> T@U!val!77
 realType -> T@T!val!1
 refType -> T@T!val!16
 regexType -> T@T!val!5
+remainingString##1_0 -> 
+remainingString##2_0 -> 
+remainingString#0@@5 -> T@U!val!74
 rmodeType -> T@T!val!3
 stringType -> T@T!val!4
 TagBool -> T@U!val!5
@@ -55,18 +68,21 @@ TagChar -> T@U!val!6
 TagClass -> T@U!val!16
 Tagclass._System.___hFunc0 -> T@U!val!34
 Tagclass._System.___hFunc1 -> T@U!val!31
+Tagclass._System.___hFunc3 -> T@U!val!37
 Tagclass._System.___hPartialFunc0 -> T@U!val!35
 Tagclass._System.___hPartialFunc1 -> T@U!val!32
+Tagclass._System.___hPartialFunc3 -> T@U!val!38
 Tagclass._System.___hTotalFunc0 -> T@U!val!36
 Tagclass._System.___hTotalFunc1 -> T@U!val!33
+Tagclass._System.___hTotalFunc3 -> T@U!val!39
 Tagclass._System.array -> T@U!val!30
 Tagclass._System.array? -> T@U!val!29
 Tagclass._System.nat -> T@U!val!24
 Tagclass._System.object -> T@U!val!27
 Tagclass._System.object? -> T@U!val!26
-Tagclass._System.Tuple0 -> T@U!val!41
-Tagclass._System.Tuple2 -> T@U!val!38
-Tagclass.M.__default -> T@U!val!44
+Tagclass._System.Tuple0 -> T@U!val!44
+Tagclass._System.Tuple2 -> T@U!val!41
+Tagclass.M.__default -> T@U!val!47
 TagIMap -> T@U!val!15
 TagInt -> T@U!val!7
 TagISet -> T@U!val!11
@@ -78,86 +94,95 @@ TagSeq -> T@U!val!13
 TagSet -> T@U!val!10
 TBool -> T@U!val!0
 TChar -> T@U!val!1
-Tclass._System.nat -> T@U!val!59
-Tclass._System.object -> T@U!val!61
-Tclass._System.object? -> T@U!val!57
-Tclass._System.Tuple0 -> T@U!val!62
-Tclass.M.__default -> T@U!val!64
+Tclass._System.nat -> T@U!val!65
+Tclass._System.object -> T@U!val!67
+Tclass._System.object? -> T@U!val!63
+Tclass._System.Tuple0 -> T@U!val!68
+Tclass.M.__default -> T@U!val!70
 TInt -> T@U!val!2
 TORDINAL -> T@U!val!4
 TReal -> T@U!val!3
-tytagFamily$_#Func0 -> T@U!val!51
-tytagFamily$_#Func1 -> T@U!val!48
-tytagFamily$_#PartialFunc0 -> T@U!val!52
-tytagFamily$_#PartialFunc1 -> T@U!val!49
-tytagFamily$_#TotalFunc0 -> T@U!val!53
-tytagFamily$_#TotalFunc1 -> T@U!val!50
-tytagFamily$_default -> T@U!val!56
-tytagFamily$_tuple#0 -> T@U!val!55
-tytagFamily$_tuple#2 -> T@U!val!54
-tytagFamily$array -> T@U!val!47
-tytagFamily$nat -> T@U!val!45
-tytagFamily$object -> T@U!val!46
+tytagFamily$_#Func0 -> T@U!val!54
+tytagFamily$_#Func1 -> T@U!val!51
+tytagFamily$_#Func3 -> T@U!val!57
+tytagFamily$_#PartialFunc0 -> T@U!val!55
+tytagFamily$_#PartialFunc1 -> T@U!val!52
+tytagFamily$_#PartialFunc3 -> T@U!val!58
+tytagFamily$_#TotalFunc0 -> T@U!val!56
+tytagFamily$_#TotalFunc1 -> T@U!val!53
+tytagFamily$_#TotalFunc3 -> T@U!val!59
+tytagFamily$_default -> T@U!val!62
+tytagFamily$_tuple#0 -> T@U!val!61
+tytagFamily$_tuple#2 -> T@U!val!60
+tytagFamily$array -> T@U!val!50
+tytagFamily$nat -> T@U!val!48
+tytagFamily$object -> T@U!val!49
 TyTagFamilyType -> T@T!val!12
 TyTagType -> T@T!val!7
 TyType -> T@T!val!6
-unique-value!100 -> distinct-elems!84!val!14
-unique-value!101 -> distinct-elems!84!val!15
-unique-value!102 -> distinct-elems!84!val!16
-unique-value!103 -> distinct-elems!84!val!17
-unique-value!104 -> distinct-elems!84!val!18
-unique-value!105 -> distinct-elems!84!val!19
-unique-value!106 -> distinct-elems!84!val!20
-unique-value!107 -> distinct-elems!84!val!21
-unique-value!108 -> distinct-elems!84!val!22
-unique-value!109 -> distinct-elems!84!val!23
-unique-value!110 -> distinct-elems!84!val!24
-unique-value!111 -> distinct-elems!84!val!25
-unique-value!112 -> distinct-elems!84!val!26
-unique-value!113 -> distinct-elems!84!val!27
-unique-value!114 -> distinct-elems!84!val!28
-unique-value!115 -> distinct-elems!84!val!29
-unique-value!116 -> distinct-elems!84!val!30
-unique-value!117 -> distinct-elems!84!val!31
-unique-value!118 -> distinct-elems!84!val!32
-unique-value!119 -> distinct-elems!84!val!33
-unique-value!120 -> distinct-elems!84!val!34
-unique-value!121 -> distinct-elems!84!val!35
-unique-value!122 -> distinct-elems!84!val!36
-unique-value!123 -> distinct-elems!84!val!37
-unique-value!124 -> distinct-elems!84!val!38
-unique-value!125 -> distinct-elems!84!val!39
-unique-value!126 -> distinct-elems!84!val!40
-unique-value!127 -> distinct-elems!84!val!41
-unique-value!128 -> distinct-elems!84!val!42
-unique-value!129 -> distinct-elems!84!val!43
-unique-value!130 -> distinct-elems!84!val!44
-unique-value!131 -> distinct-elems!84!val!45
-unique-value!132 -> distinct-elems!84!val!46
-unique-value!133 -> distinct-elems!84!val!47
-unique-value!134 -> distinct-elems!84!val!48
-unique-value!135 -> distinct-elems!84!val!49
-unique-value!136 -> distinct-elems!84!val!50
-unique-value!137 -> distinct-elems!84!val!51
-unique-value!138 -> distinct-elems!84!val!52
-unique-value!139 -> distinct-elems!84!val!53
-unique-value!140 -> distinct-elems!84!val!54
-unique-value!141 -> distinct-elems!84!val!55
-unique-value!142 -> distinct-elems!84!val!56
-unique-value!86 -> distinct-elems!84!val!0
-unique-value!87 -> distinct-elems!84!val!1
-unique-value!88 -> distinct-elems!84!val!2
-unique-value!89 -> distinct-elems!84!val!3
-unique-value!90 -> distinct-elems!84!val!4
-unique-value!91 -> distinct-elems!84!val!5
-unique-value!92 -> distinct-elems!84!val!6
-unique-value!93 -> distinct-elems!84!val!7
-unique-value!94 -> distinct-elems!84!val!8
-unique-value!95 -> distinct-elems!84!val!9
-unique-value!96 -> distinct-elems!84!val!10
-unique-value!97 -> distinct-elems!84!val!11
-unique-value!98 -> distinct-elems!84!val!12
-unique-value!99 -> distinct-elems!84!val!13
+unique-value!116 -> distinct-elems!114!val!0
+unique-value!117 -> distinct-elems!114!val!1
+unique-value!118 -> distinct-elems!114!val!2
+unique-value!119 -> distinct-elems!114!val!3
+unique-value!120 -> distinct-elems!114!val!4
+unique-value!121 -> distinct-elems!114!val!5
+unique-value!122 -> distinct-elems!114!val!6
+unique-value!123 -> distinct-elems!114!val!7
+unique-value!124 -> distinct-elems!114!val!8
+unique-value!125 -> distinct-elems!114!val!9
+unique-value!126 -> distinct-elems!114!val!10
+unique-value!127 -> distinct-elems!114!val!11
+unique-value!128 -> distinct-elems!114!val!12
+unique-value!129 -> distinct-elems!114!val!13
+unique-value!130 -> distinct-elems!114!val!14
+unique-value!131 -> distinct-elems!114!val!15
+unique-value!132 -> distinct-elems!114!val!16
+unique-value!133 -> distinct-elems!114!val!17
+unique-value!134 -> distinct-elems!114!val!18
+unique-value!135 -> distinct-elems!114!val!19
+unique-value!136 -> distinct-elems!114!val!20
+unique-value!137 -> distinct-elems!114!val!21
+unique-value!138 -> distinct-elems!114!val!22
+unique-value!139 -> distinct-elems!114!val!23
+unique-value!140 -> distinct-elems!114!val!24
+unique-value!141 -> distinct-elems!114!val!25
+unique-value!142 -> distinct-elems!114!val!26
+unique-value!143 -> distinct-elems!114!val!27
+unique-value!144 -> distinct-elems!114!val!28
+unique-value!145 -> distinct-elems!114!val!29
+unique-value!146 -> distinct-elems!114!val!30
+unique-value!147 -> distinct-elems!114!val!31
+unique-value!148 -> distinct-elems!114!val!32
+unique-value!149 -> distinct-elems!114!val!33
+unique-value!150 -> distinct-elems!114!val!34
+unique-value!151 -> distinct-elems!114!val!35
+unique-value!152 -> distinct-elems!114!val!36
+unique-value!153 -> distinct-elems!114!val!37
+unique-value!154 -> distinct-elems!114!val!38
+unique-value!155 -> distinct-elems!114!val!39
+unique-value!156 -> distinct-elems!114!val!40
+unique-value!157 -> distinct-elems!114!val!41
+unique-value!158 -> distinct-elems!114!val!42
+unique-value!159 -> distinct-elems!114!val!43
+unique-value!160 -> distinct-elems!114!val!44
+unique-value!161 -> distinct-elems!114!val!45
+unique-value!162 -> distinct-elems!114!val!46
+unique-value!163 -> distinct-elems!114!val!47
+unique-value!164 -> distinct-elems!114!val!48
+unique-value!165 -> distinct-elems!114!val!49
+unique-value!166 -> distinct-elems!114!val!50
+unique-value!167 -> distinct-elems!114!val!51
+unique-value!168 -> distinct-elems!114!val!52
+unique-value!169 -> distinct-elems!114!val!53
+unique-value!170 -> distinct-elems!114!val!54
+unique-value!171 -> distinct-elems!114!val!55
+unique-value!172 -> distinct-elems!114!val!56
+unique-value!173 -> distinct-elems!114!val!57
+unique-value!174 -> distinct-elems!114!val!58
+unique-value!175 -> distinct-elems!114!val!59
+unique-value!176 -> distinct-elems!114!val!60
+unique-value!177 -> distinct-elems!114!val!61
+unique-value!178 -> distinct-elems!114!val!62
 _System.array.Length -> {
   else -> 0
 }
@@ -192,7 +217,15 @@ $HeapSuccGhost -> {
   else -> false
 }
 $Is -> {
-  T@U!val!63 T@U!val!62 -> true
+  T@U!val!69 T@U!val!68 -> true
+  T@U!val!73 T@U!val!82 -> true
+  T@U!val!74 T@U!val!82 -> true
+  T@U!val!75 T@U!val!82 -> true
+  T@U!val!77 T@U!val!82 -> true
+  T@U!val!78 T@U!val!82 -> true
+  T@U!val!79 T@U!val!82 -> true
+  T@U!val!80 T@U!val!82 -> true
+  T@U!val!81 T@U!val!82 -> true
   else -> true
 }
 $IsA#_System.Tuple0 -> {
@@ -202,7 +235,15 @@ $IsA#_System.Tuple2 -> {
   else -> false
 }
 $IsAlloc -> {
-  else -> false
+  T@U!val!73 T@U!val!82 T@U!val!72 -> true
+  T@U!val!74 T@U!val!82 T@U!val!72 -> true
+  T@U!val!75 T@U!val!82 T@U!val!72 -> true
+  T@U!val!77 T@U!val!82 T@U!val!72 -> true
+  T@U!val!78 T@U!val!82 T@U!val!72 -> true
+  T@U!val!79 T@U!val!82 T@U!val!72 -> true
+  T@U!val!80 T@U!val!82 T@U!val!72 -> true
+  T@U!val!81 T@U!val!82 T@U!val!72 -> true
+  else -> true
 }
 $IsAllocBox -> {
   else -> false
@@ -215,15 +256,15 @@ $IsGhostField -> {
   else -> false
 }
 $IsGoodHeap -> {
-  T@U!val!58 -> true
-  T@U!val!65 -> true
+  T@U!val!64 -> true
+  T@U!val!72 -> true
   else -> true
 }
 $IsGoodMultiSet -> {
   else -> false
 }
 $IsHeapAnchor -> {
-  T@U!val!65 -> true
+  T@U!val!72 -> true
   else -> true
 }
 $LS -> {
@@ -239,6 +280,12 @@ Apply0 -> {
   else -> T@U!val!0
 }
 Apply1 -> {
+  else -> T@U!val!0
+}
+Apply3 -> {
+  else -> T@U!val!0
+}
+AsFuelBottom -> {
   else -> T@U!val!0
 }
 AtLayer -> {
@@ -264,10 +311,10 @@ char#ToInt -> {
   else -> 0
 }
 ControlFlow -> {
-  0 0 -> 63373
-  0 54326 -> (- 63445)
-  0 63373 -> 54326
-  else -> 63373
+  0 0 -> 123963
+  0 123963 -> 70422
+  0 70422 -> (- 124257)
+  else -> 123963
 }
 Ctor -> {
   T@T!val!0 -> 0
@@ -284,7 +331,8 @@ Ctor -> {
   T@T!val!19 -> 15
   T@T!val!2 -> 2
   T@T!val!20 -> 23
-  T@T!val!21 -> 25
+  T@T!val!21 -> 26
+  T@T!val!22 -> 16
   T@T!val!3 -> 3
   T@T!val!4 -> 4
   T@T!val!5 -> 5
@@ -295,8 +343,8 @@ Ctor -> {
   else -> 0
 }
 DatatypeCtorId -> {
-  T@U!val!63 -> T@U!val!40
-  else -> T@U!val!40
+  T@U!val!69 -> T@U!val!43
+  else -> T@U!val!43
 }
 DeclName -> {
   T@U!val!22 -> T@U!val!23
@@ -305,65 +353,71 @@ DeclName -> {
 DeclType -> {
   else -> T@U!val!0
 }
-distinct-aux-f!!85 -> {
-  T@U!val!0 -> distinct-elems!84!val!0
-  T@U!val!1 -> distinct-elems!84!val!1
-  T@U!val!10 -> distinct-elems!84!val!10
-  T@U!val!11 -> distinct-elems!84!val!11
-  T@U!val!12 -> distinct-elems!84!val!12
-  T@U!val!13 -> distinct-elems!84!val!13
-  T@U!val!14 -> distinct-elems!84!val!14
-  T@U!val!15 -> distinct-elems!84!val!15
-  T@U!val!16 -> distinct-elems!84!val!16
-  T@U!val!17 -> distinct-elems!84!val!17
-  T@U!val!18 -> distinct-elems!84!val!18
-  T@U!val!19 -> distinct-elems!84!val!19
-  T@U!val!2 -> distinct-elems!84!val!2
-  T@U!val!20 -> distinct-elems!84!val!20
-  T@U!val!21 -> distinct-elems!84!val!21
-  T@U!val!22 -> distinct-elems!84!val!22
-  T@U!val!23 -> distinct-elems!84!val!23
-  T@U!val!24 -> distinct-elems!84!val!24
-  T@U!val!25 -> distinct-elems!84!val!25
-  T@U!val!26 -> distinct-elems!84!val!26
-  T@U!val!27 -> distinct-elems!84!val!27
-  T@U!val!28 -> distinct-elems!84!val!28
-  T@U!val!29 -> distinct-elems!84!val!29
-  T@U!val!3 -> distinct-elems!84!val!3
-  T@U!val!30 -> distinct-elems!84!val!30
-  T@U!val!31 -> distinct-elems!84!val!31
-  T@U!val!32 -> distinct-elems!84!val!32
-  T@U!val!33 -> distinct-elems!84!val!33
-  T@U!val!34 -> distinct-elems!84!val!34
-  T@U!val!35 -> distinct-elems!84!val!35
-  T@U!val!36 -> distinct-elems!84!val!36
-  T@U!val!37 -> distinct-elems!84!val!37
-  T@U!val!38 -> distinct-elems!84!val!38
-  T@U!val!39 -> distinct-elems!84!val!39
-  T@U!val!4 -> distinct-elems!84!val!4
-  T@U!val!40 -> distinct-elems!84!val!40
-  T@U!val!41 -> distinct-elems!84!val!41
-  T@U!val!42 -> distinct-elems!84!val!42
-  T@U!val!43 -> distinct-elems!84!val!43
-  T@U!val!44 -> distinct-elems!84!val!44
-  T@U!val!45 -> distinct-elems!84!val!45
-  T@U!val!46 -> distinct-elems!84!val!46
-  T@U!val!47 -> distinct-elems!84!val!47
-  T@U!val!48 -> distinct-elems!84!val!48
-  T@U!val!49 -> distinct-elems!84!val!49
-  T@U!val!5 -> distinct-elems!84!val!5
-  T@U!val!50 -> distinct-elems!84!val!50
-  T@U!val!51 -> distinct-elems!84!val!51
-  T@U!val!52 -> distinct-elems!84!val!52
-  T@U!val!53 -> distinct-elems!84!val!53
-  T@U!val!54 -> distinct-elems!84!val!54
-  T@U!val!55 -> distinct-elems!84!val!55
-  T@U!val!56 -> distinct-elems!84!val!56
-  T@U!val!6 -> distinct-elems!84!val!6
-  T@U!val!7 -> distinct-elems!84!val!7
-  T@U!val!8 -> distinct-elems!84!val!8
-  T@U!val!9 -> distinct-elems!84!val!9
-  else -> distinct-elems!84!val!0
+distinct-aux-f!!115 -> {
+  T@U!val!0 -> distinct-elems!114!val!0
+  T@U!val!1 -> distinct-elems!114!val!1
+  T@U!val!10 -> distinct-elems!114!val!10
+  T@U!val!11 -> distinct-elems!114!val!11
+  T@U!val!12 -> distinct-elems!114!val!12
+  T@U!val!13 -> distinct-elems!114!val!13
+  T@U!val!14 -> distinct-elems!114!val!14
+  T@U!val!15 -> distinct-elems!114!val!15
+  T@U!val!16 -> distinct-elems!114!val!16
+  T@U!val!17 -> distinct-elems!114!val!17
+  T@U!val!18 -> distinct-elems!114!val!18
+  T@U!val!19 -> distinct-elems!114!val!19
+  T@U!val!2 -> distinct-elems!114!val!2
+  T@U!val!20 -> distinct-elems!114!val!20
+  T@U!val!21 -> distinct-elems!114!val!21
+  T@U!val!22 -> distinct-elems!114!val!22
+  T@U!val!23 -> distinct-elems!114!val!23
+  T@U!val!24 -> distinct-elems!114!val!24
+  T@U!val!25 -> distinct-elems!114!val!25
+  T@U!val!26 -> distinct-elems!114!val!26
+  T@U!val!27 -> distinct-elems!114!val!27
+  T@U!val!28 -> distinct-elems!114!val!28
+  T@U!val!29 -> distinct-elems!114!val!29
+  T@U!val!3 -> distinct-elems!114!val!3
+  T@U!val!30 -> distinct-elems!114!val!30
+  T@U!val!31 -> distinct-elems!114!val!31
+  T@U!val!32 -> distinct-elems!114!val!32
+  T@U!val!33 -> distinct-elems!114!val!33
+  T@U!val!34 -> distinct-elems!114!val!34
+  T@U!val!35 -> distinct-elems!114!val!35
+  T@U!val!36 -> distinct-elems!114!val!36
+  T@U!val!37 -> distinct-elems!114!val!37
+  T@U!val!38 -> distinct-elems!114!val!38
+  T@U!val!39 -> distinct-elems!114!val!39
+  T@U!val!4 -> distinct-elems!114!val!4
+  T@U!val!40 -> distinct-elems!114!val!40
+  T@U!val!41 -> distinct-elems!114!val!41
+  T@U!val!42 -> distinct-elems!114!val!42
+  T@U!val!43 -> distinct-elems!114!val!43
+  T@U!val!44 -> distinct-elems!114!val!44
+  T@U!val!45 -> distinct-elems!114!val!45
+  T@U!val!46 -> distinct-elems!114!val!46
+  T@U!val!47 -> distinct-elems!114!val!47
+  T@U!val!48 -> distinct-elems!114!val!48
+  T@U!val!49 -> distinct-elems!114!val!49
+  T@U!val!5 -> distinct-elems!114!val!5
+  T@U!val!50 -> distinct-elems!114!val!50
+  T@U!val!51 -> distinct-elems!114!val!51
+  T@U!val!52 -> distinct-elems!114!val!52
+  T@U!val!53 -> distinct-elems!114!val!53
+  T@U!val!54 -> distinct-elems!114!val!54
+  T@U!val!55 -> distinct-elems!114!val!55
+  T@U!val!56 -> distinct-elems!114!val!56
+  T@U!val!57 -> distinct-elems!114!val!57
+  T@U!val!58 -> distinct-elems!114!val!58
+  T@U!val!59 -> distinct-elems!114!val!59
+  T@U!val!6 -> distinct-elems!114!val!6
+  T@U!val!60 -> distinct-elems!114!val!60
+  T@U!val!61 -> distinct-elems!114!val!61
+  T@U!val!62 -> distinct-elems!114!val!62
+  T@U!val!7 -> distinct-elems!114!val!7
+  T@U!val!8 -> distinct-elems!114!val!8
+  T@U!val!9 -> distinct-elems!114!val!9
+  else -> distinct-elems!114!val!0
 }
 Div -> {
   else -> 0
@@ -393,6 +447,9 @@ Handle0 -> {
   else -> T@U!val!0
 }
 Handle1 -> {
+  else -> T@U!val!0
+}
+Handle3 -> {
   else -> T@U!val!0
 }
 IMap#Build -> {
@@ -486,7 +543,8 @@ Inv0_TMultiSet -> {
   else -> T@U!val!0
 }
 Inv0_TSeq -> {
-  else -> T@U!val!0
+  T@U!val!82 -> T@U!val!1
+  else -> T@U!val!1
 }
 Inv0_TSet -> {
   else -> T@U!val!0
@@ -522,19 +580,38 @@ ISet#UnionOne -> {
   else -> T@U!val!0
 }
 lambda#0 -> {
-  T@U!val!60 T@U!val!65 T@U!val!22 false -> T@U!val!66
-  else -> T@U!val!66
+  else -> T@U!val!0
+}
+lambda#1 -> {
+  else -> T@U!val!0
+}
+lambda#2 -> {
+  else -> T@U!val!0
+}
+lambda#3 -> {
+  T@U!val!66 T@U!val!72 T@U!val!22 false -> T@U!val!83
+  else -> T@U!val!83
 }
 Lit -> {
   false -> false
-  T@U!val!63 -> T@U!val!63
-  else -> T@U!val!63
+  T@U!val!69 -> T@U!val!69
+  else -> T@U!val!69
 }
 LitInt -> {
+  0 -> 0
   else -> 0
 }
 LitReal -> {
   else -> 0.0
+}
+M.__default.replaceRecursiveFunc -> {
+  else -> T@U!val!0
+}
+M.__default.replaceRecursiveFunc#canCall -> {
+  else -> false
+}
+M.__default.replaceRecursiveFunc#requires -> {
+  else -> false
 }
 Map#Build -> {
   else -> T@U!val!0
@@ -624,14 +701,38 @@ MapType3Store -> {
   else -> T@U!val!0
 }
 MapType3Type -> {
+  else -> T@T!val!0
+}
+MapType3TypeInv0 -> {
+  else -> T@T!val!0
+}
+MapType3TypeInv1 -> {
+  else -> T@T!val!0
+}
+MapType3TypeInv2 -> {
+  else -> T@T!val!0
+}
+MapType3TypeInv3 -> {
+  else -> T@T!val!0
+}
+MapType3TypeInv4 -> {
+  else -> T@T!val!0
+}
+MapType4Select -> {
+  else -> T@U!val!0
+}
+MapType4Store -> {
+  else -> T@U!val!0
+}
+MapType4Type -> {
   T@T!val!16 T@T!val!2 -> T@T!val!21
   else -> T@T!val!21
 }
-MapType3TypeInv0 -> {
+MapType4TypeInv0 -> {
   T@T!val!21 -> T@T!val!16
   else -> T@T!val!16
 }
-MapType3TypeInv1 -> {
+MapType4TypeInv1 -> {
   T@T!val!21 -> T@T!val!2
   else -> T@T!val!2
 }
@@ -731,6 +832,9 @@ Reads0 -> {
 Reads1 -> {
   else -> T@U!val!0
 }
+Reads3 -> {
+  else -> T@U!val!0
+}
 real_2_U -> {
   else -> T@U!val!0
 }
@@ -744,6 +848,9 @@ Requires0 -> {
   else -> false
 }
 Requires1 -> {
+  else -> false
+}
+Requires3 -> {
   else -> false
 }
 rmode_2_U -> {
@@ -783,7 +890,10 @@ Seq#Index -> {
   else -> T@U!val!0
 }
 Seq#Length -> {
-  else -> 0
+  T@U!val!73 -> 1
+  T@U!val!74 -> 1
+  T@U!val!75 -> 1
+  else -> 1
 }
 Seq#Rank -> {
   else -> 0
@@ -801,10 +911,12 @@ Seq#Update -> {
   else -> T@U!val!0
 }
 SeqType -> {
-  else -> T@T!val!0
+  T@T!val!13 -> T@T!val!22
+  else -> T@T!val!22
 }
 SeqTypeInv0 -> {
-  else -> T@T!val!0
+  T@T!val!22 -> T@T!val!13
+  else -> T@T!val!13
 }
 Set#Card -> {
   else -> 0
@@ -851,20 +963,21 @@ Tag -> {
   T@U!val!2 -> T@U!val!7
   T@U!val!3 -> T@U!val!8
   T@U!val!4 -> T@U!val!9
-  T@U!val!57 -> T@U!val!26
-  T@U!val!59 -> T@U!val!24
-  T@U!val!61 -> T@U!val!27
-  T@U!val!62 -> T@U!val!41
-  T@U!val!64 -> T@U!val!44
+  T@U!val!63 -> T@U!val!26
+  T@U!val!65 -> T@U!val!24
+  T@U!val!67 -> T@U!val!27
+  T@U!val!68 -> T@U!val!44
+  T@U!val!70 -> T@U!val!47
+  T@U!val!82 -> T@U!val!13
   else -> T@U!val!5
 }
 TagFamily -> {
-  T@U!val!57 -> T@U!val!46
-  T@U!val!59 -> T@U!val!45
-  T@U!val!61 -> T@U!val!46
-  T@U!val!62 -> T@U!val!55
-  T@U!val!64 -> T@U!val!56
-  else -> T@U!val!46
+  T@U!val!63 -> T@U!val!49
+  T@U!val!65 -> T@U!val!48
+  T@U!val!67 -> T@U!val!49
+  T@U!val!68 -> T@U!val!61
+  T@U!val!70 -> T@U!val!62
+  else -> T@U!val!49
 }
 TBitvector -> {
   else -> T@U!val!0
@@ -884,6 +997,21 @@ Tclass._System.___hFunc1_0 -> {
 Tclass._System.___hFunc1_1 -> {
   else -> T@U!val!0
 }
+Tclass._System.___hFunc3 -> {
+  else -> T@U!val!0
+}
+Tclass._System.___hFunc3_0 -> {
+  else -> T@U!val!0
+}
+Tclass._System.___hFunc3_1 -> {
+  else -> T@U!val!0
+}
+Tclass._System.___hFunc3_2 -> {
+  else -> T@U!val!0
+}
+Tclass._System.___hFunc3_3 -> {
+  else -> T@U!val!0
+}
 Tclass._System.___hPartialFunc0 -> {
   else -> T@U!val!0
 }
@@ -899,6 +1027,21 @@ Tclass._System.___hPartialFunc1_0 -> {
 Tclass._System.___hPartialFunc1_1 -> {
   else -> T@U!val!0
 }
+Tclass._System.___hPartialFunc3 -> {
+  else -> T@U!val!0
+}
+Tclass._System.___hPartialFunc3_0 -> {
+  else -> T@U!val!0
+}
+Tclass._System.___hPartialFunc3_1 -> {
+  else -> T@U!val!0
+}
+Tclass._System.___hPartialFunc3_2 -> {
+  else -> T@U!val!0
+}
+Tclass._System.___hPartialFunc3_3 -> {
+  else -> T@U!val!0
+}
 Tclass._System.___hTotalFunc0 -> {
   else -> T@U!val!0
 }
@@ -912,6 +1055,21 @@ Tclass._System.___hTotalFunc1_0 -> {
   else -> T@U!val!0
 }
 Tclass._System.___hTotalFunc1_1 -> {
+  else -> T@U!val!0
+}
+Tclass._System.___hTotalFunc3 -> {
+  else -> T@U!val!0
+}
+Tclass._System.___hTotalFunc3_0 -> {
+  else -> T@U!val!0
+}
+Tclass._System.___hTotalFunc3_1 -> {
+  else -> T@U!val!0
+}
+Tclass._System.___hTotalFunc3_2 -> {
+  else -> T@U!val!0
+}
+Tclass._System.___hTotalFunc3_3 -> {
   else -> T@U!val!0
 }
 Tclass._System.array -> {
@@ -953,7 +1111,8 @@ TMultiSet -> {
   else -> T@U!val!0
 }
 TSeq -> {
-  else -> T@U!val!0
+  T@U!val!1 -> T@U!val!82
+  else -> T@U!val!82
 }
 TSet -> {
   else -> T@U!val!0
@@ -991,18 +1150,18 @@ type -> {
   T@U!val!34 -> T@T!val!7
   T@U!val!35 -> T@T!val!7
   T@U!val!36 -> T@T!val!7
-  T@U!val!37 -> T@T!val!11
+  T@U!val!37 -> T@T!val!7
   T@U!val!38 -> T@T!val!7
-  T@U!val!39 -> T@T!val!8
+  T@U!val!39 -> T@T!val!7
   T@U!val!4 -> T@T!val!6
   T@U!val!40 -> T@T!val!11
   T@U!val!41 -> T@T!val!7
   T@U!val!42 -> T@T!val!8
-  T@U!val!43 -> T@T!val!8
+  T@U!val!43 -> T@T!val!11
   T@U!val!44 -> T@T!val!7
-  T@U!val!45 -> T@T!val!12
-  T@U!val!46 -> T@T!val!12
-  T@U!val!47 -> T@T!val!12
+  T@U!val!45 -> T@T!val!8
+  T@U!val!46 -> T@T!val!8
+  T@U!val!47 -> T@T!val!7
   T@U!val!48 -> T@T!val!12
   T@U!val!49 -> T@T!val!12
   T@U!val!5 -> T@T!val!7
@@ -1013,19 +1172,36 @@ type -> {
   T@U!val!54 -> T@T!val!12
   T@U!val!55 -> T@T!val!12
   T@U!val!56 -> T@T!val!12
-  T@U!val!57 -> T@T!val!6
-  T@U!val!58 -> T@T!val!19
-  T@U!val!59 -> T@T!val!6
+  T@U!val!57 -> T@T!val!12
+  T@U!val!58 -> T@T!val!12
+  T@U!val!59 -> T@T!val!12
   T@U!val!6 -> T@T!val!7
-  T@U!val!60 -> T@T!val!16
-  T@U!val!61 -> T@T!val!6
-  T@U!val!62 -> T@T!val!6
-  T@U!val!63 -> T@T!val!17
-  T@U!val!64 -> T@T!val!6
-  T@U!val!65 -> T@T!val!19
-  T@U!val!66 -> T@T!val!21
+  T@U!val!60 -> T@T!val!12
+  T@U!val!61 -> T@T!val!12
+  T@U!val!62 -> T@T!val!12
+  T@U!val!63 -> T@T!val!6
+  T@U!val!64 -> T@T!val!19
+  T@U!val!65 -> T@T!val!6
+  T@U!val!66 -> T@T!val!16
+  T@U!val!67 -> T@T!val!6
+  T@U!val!68 -> T@T!val!6
+  T@U!val!69 -> T@T!val!17
   T@U!val!7 -> T@T!val!7
+  T@U!val!70 -> T@T!val!6
+  T@U!val!71 -> T@T!val!18
+  T@U!val!72 -> T@T!val!19
+  T@U!val!73 -> T@T!val!22
+  T@U!val!74 -> T@T!val!22
+  T@U!val!75 -> T@T!val!22
+  T@U!val!76 -> T@T!val!22
+  T@U!val!77 -> T@T!val!22
+  T@U!val!78 -> T@T!val!22
+  T@U!val!79 -> T@T!val!22
   T@U!val!8 -> T@T!val!7
+  T@U!val!80 -> T@T!val!22
+  T@U!val!81 -> T@T!val!22
+  T@U!val!82 -> T@T!val!6
+  T@U!val!83 -> T@T!val!21
   T@U!val!9 -> T@T!val!7
   else -> T@T!val!7
 }
@@ -1066,44 +1242,56 @@ UOrdering3 -> {
 *** STATE <initial>
   $_Frame -> 
   $_reverifyPost -> 
-  $Heap -> T@U!val!65
+  $Heap -> T@U!val!72
+  $rhs##1_0 -> T@U!val!78
+  $rhs##2_0 -> T@U!val!81
   $Tick -> 
-  a#0 -> 11
-  b#0 -> 6
-  c#0 -> 
-  defass#c#0 -> 
+  defass#newString#0 -> false
+  first#2_0 -> T@U!val!79
+  inner#2_0 -> T@U!val!80
+  newString#0 -> T@U!val!76
+  other##1_0 -> 
+  other##2_0 -> 
+  other#0 -> T@U!val!75
+  pattern##1_0 -> 
+  pattern##2_0 -> 
+  pattern#0 -> T@U!val!73
+  prefixedInner#1_0 -> T@U!val!77
+  remainingString##1_0 -> 
+  remainingString##2_0 -> 
+  remainingString#0 -> T@U!val!74
 *** END_STATE
-*** STATE /workspaces/dafny/string_project/str_recurse.dfy(5,2): initial state
-  $_Frame -> T@U!val!66
+*** STATE /workspaces/dafny/string_project/str_recurse.dfy(35,2): initial state
+  $_Frame -> T@U!val!83
 *** END_STATE
 *** END_MODEL
-<no file>(1500,4): Error: This assertion might not hold.
+<no file>(1823,4): Error: This assertion might not hold.
 Execution trace:
-    (1609,3): anon0
+    (1981,3): anon0
 Augmented execution trace:
-Impl | Impl$$M.__default.foo | 11 | 5
-Types | int | int
+Impl | Impl$$M.__default.replaceRecursive | T@U!val!73 | T@U!val!84 | T@U!val!74
+Types | Seq Box | Seq Box | Seq Box
 
 
 *** MODEL
-#_System._tuple#0._#Make0 -> T@U!val!63
-##_System._tuple#0._#Make0 -> T@U!val!40
-##_System._tuple#2._#Make2 -> T@U!val!37
+#_System._tuple#0._#Make0 -> T@U!val!69
+##_System._tuple#0._#Make0 -> T@U!val!43
+##_System._tuple#2._#Make2 -> T@U!val!40
 $_Frame -> 
-$_Frame@0 -> T@U!val!66
+$_Frame@0 -> T@U!val!82
 $_reverifyPost -> 
 $$Language$Dafny -> true
-$FunctionContextHeight -> 0
-$Heap -> T@U!val!65
-$OneHeap -> T@U!val!58
+$FunctionContextHeight -> 2
+$Heap -> T@U!val!72
+$LZ -> T@U!val!71
+$OneHeap -> T@U!val!64
+$rhs##1_0 -> T@U!val!77
+$rhs##2_0 -> T@U!val!80
 $Tick -> 
-a#0 -> 11
 alloc -> T@U!val!22
 allocName -> T@U!val!23
-b#0 -> 5
 boolType -> T@T!val!2
 BoxType -> T@T!val!13
-c#0 -> 
 charType -> T@T!val!14
 class._System.array? -> T@U!val!28
 class._System.bool -> T@U!val!18
@@ -1112,23 +1300,36 @@ class._System.multiset -> T@U!val!21
 class._System.object? -> T@U!val!25
 class._System.seq -> T@U!val!20
 class._System.set -> T@U!val!19
-class._System.Tuple0 -> T@U!val!42
-class._System.Tuple2 -> T@U!val!39
-class.M.__default -> T@U!val!43
+class._System.Tuple0 -> T@U!val!45
+class._System.Tuple2 -> T@U!val!42
+class.M.__default -> T@U!val!46
 ClassNameType -> T@T!val!8
 DatatypeTypeType -> T@T!val!17
-defass#c#0 -> 
+defass#newString#0 -> false
 DtCtorIdType -> T@T!val!11
+first#2_0 -> T@U!val!78
 HandleTypeType -> T@T!val!20
+inner#2_0 -> T@U!val!79
 intType -> T@T!val!0
 LayerTypeType -> T@T!val!18
 MapType1Type -> T@T!val!15
 NameFamilyType -> T@T!val!10
-null -> T@U!val!60
-proxy!143 -> true
+newString#0 -> T@U!val!75
+null -> T@U!val!66
+other##1_0 -> 
+other##2_0 -> 
+other#0@@5 -> T@U!val!74
+pattern##1_0 -> 
+pattern##2_0 -> 
+pattern#0@@5 -> T@U!val!84
+prefixedInner#1_0 -> T@U!val!76
+proxy!179 -> true
 realType -> T@T!val!1
 refType -> T@T!val!16
 regexType -> T@T!val!5
+remainingString##1_0 -> 
+remainingString##2_0 -> 
+remainingString#0@@5 -> T@U!val!73
 rmodeType -> T@T!val!3
 stringType -> T@T!val!4
 TagBool -> T@U!val!5
@@ -1136,18 +1337,21 @@ TagChar -> T@U!val!6
 TagClass -> T@U!val!16
 Tagclass._System.___hFunc0 -> T@U!val!34
 Tagclass._System.___hFunc1 -> T@U!val!31
+Tagclass._System.___hFunc3 -> T@U!val!37
 Tagclass._System.___hPartialFunc0 -> T@U!val!35
 Tagclass._System.___hPartialFunc1 -> T@U!val!32
+Tagclass._System.___hPartialFunc3 -> T@U!val!38
 Tagclass._System.___hTotalFunc0 -> T@U!val!36
 Tagclass._System.___hTotalFunc1 -> T@U!val!33
+Tagclass._System.___hTotalFunc3 -> T@U!val!39
 Tagclass._System.array -> T@U!val!30
 Tagclass._System.array? -> T@U!val!29
 Tagclass._System.nat -> T@U!val!24
 Tagclass._System.object -> T@U!val!27
 Tagclass._System.object? -> T@U!val!26
-Tagclass._System.Tuple0 -> T@U!val!41
-Tagclass._System.Tuple2 -> T@U!val!38
-Tagclass.M.__default -> T@U!val!44
+Tagclass._System.Tuple0 -> T@U!val!44
+Tagclass._System.Tuple2 -> T@U!val!41
+Tagclass.M.__default -> T@U!val!47
 TagIMap -> T@U!val!15
 TagInt -> T@U!val!7
 TagISet -> T@U!val!11
@@ -1159,86 +1363,95 @@ TagSeq -> T@U!val!13
 TagSet -> T@U!val!10
 TBool -> T@U!val!0
 TChar -> T@U!val!1
-Tclass._System.nat -> T@U!val!59
-Tclass._System.object -> T@U!val!61
-Tclass._System.object? -> T@U!val!57
-Tclass._System.Tuple0 -> T@U!val!62
-Tclass.M.__default -> T@U!val!64
+Tclass._System.nat -> T@U!val!65
+Tclass._System.object -> T@U!val!67
+Tclass._System.object? -> T@U!val!63
+Tclass._System.Tuple0 -> T@U!val!68
+Tclass.M.__default -> T@U!val!70
 TInt -> T@U!val!2
 TORDINAL -> T@U!val!4
 TReal -> T@U!val!3
-tytagFamily$_#Func0 -> T@U!val!51
-tytagFamily$_#Func1 -> T@U!val!48
-tytagFamily$_#PartialFunc0 -> T@U!val!52
-tytagFamily$_#PartialFunc1 -> T@U!val!49
-tytagFamily$_#TotalFunc0 -> T@U!val!53
-tytagFamily$_#TotalFunc1 -> T@U!val!50
-tytagFamily$_default -> T@U!val!56
-tytagFamily$_tuple#0 -> T@U!val!55
-tytagFamily$_tuple#2 -> T@U!val!54
-tytagFamily$array -> T@U!val!47
-tytagFamily$nat -> T@U!val!45
-tytagFamily$object -> T@U!val!46
+tytagFamily$_#Func0 -> T@U!val!54
+tytagFamily$_#Func1 -> T@U!val!51
+tytagFamily$_#Func3 -> T@U!val!57
+tytagFamily$_#PartialFunc0 -> T@U!val!55
+tytagFamily$_#PartialFunc1 -> T@U!val!52
+tytagFamily$_#PartialFunc3 -> T@U!val!58
+tytagFamily$_#TotalFunc0 -> T@U!val!56
+tytagFamily$_#TotalFunc1 -> T@U!val!53
+tytagFamily$_#TotalFunc3 -> T@U!val!59
+tytagFamily$_default -> T@U!val!62
+tytagFamily$_tuple#0 -> T@U!val!61
+tytagFamily$_tuple#2 -> T@U!val!60
+tytagFamily$array -> T@U!val!50
+tytagFamily$nat -> T@U!val!48
+tytagFamily$object -> T@U!val!49
 TyTagFamilyType -> T@T!val!12
 TyTagType -> T@T!val!7
 TyType -> T@T!val!6
-unique-value!100 -> distinct-elems!84!val!14
-unique-value!101 -> distinct-elems!84!val!15
-unique-value!102 -> distinct-elems!84!val!16
-unique-value!103 -> distinct-elems!84!val!17
-unique-value!104 -> distinct-elems!84!val!18
-unique-value!105 -> distinct-elems!84!val!19
-unique-value!106 -> distinct-elems!84!val!20
-unique-value!107 -> distinct-elems!84!val!21
-unique-value!108 -> distinct-elems!84!val!22
-unique-value!109 -> distinct-elems!84!val!23
-unique-value!110 -> distinct-elems!84!val!24
-unique-value!111 -> distinct-elems!84!val!25
-unique-value!112 -> distinct-elems!84!val!26
-unique-value!113 -> distinct-elems!84!val!27
-unique-value!114 -> distinct-elems!84!val!28
-unique-value!115 -> distinct-elems!84!val!29
-unique-value!116 -> distinct-elems!84!val!30
-unique-value!117 -> distinct-elems!84!val!31
-unique-value!118 -> distinct-elems!84!val!32
-unique-value!119 -> distinct-elems!84!val!33
-unique-value!120 -> distinct-elems!84!val!34
-unique-value!121 -> distinct-elems!84!val!35
-unique-value!122 -> distinct-elems!84!val!36
-unique-value!123 -> distinct-elems!84!val!37
-unique-value!124 -> distinct-elems!84!val!38
-unique-value!125 -> distinct-elems!84!val!39
-unique-value!126 -> distinct-elems!84!val!40
-unique-value!127 -> distinct-elems!84!val!41
-unique-value!128 -> distinct-elems!84!val!42
-unique-value!129 -> distinct-elems!84!val!43
-unique-value!130 -> distinct-elems!84!val!44
-unique-value!131 -> distinct-elems!84!val!45
-unique-value!132 -> distinct-elems!84!val!46
-unique-value!133 -> distinct-elems!84!val!47
-unique-value!134 -> distinct-elems!84!val!48
-unique-value!135 -> distinct-elems!84!val!49
-unique-value!136 -> distinct-elems!84!val!50
-unique-value!137 -> distinct-elems!84!val!51
-unique-value!138 -> distinct-elems!84!val!52
-unique-value!139 -> distinct-elems!84!val!53
-unique-value!140 -> distinct-elems!84!val!54
-unique-value!141 -> distinct-elems!84!val!55
-unique-value!142 -> distinct-elems!84!val!56
-unique-value!86 -> distinct-elems!84!val!0
-unique-value!87 -> distinct-elems!84!val!1
-unique-value!88 -> distinct-elems!84!val!2
-unique-value!89 -> distinct-elems!84!val!3
-unique-value!90 -> distinct-elems!84!val!4
-unique-value!91 -> distinct-elems!84!val!5
-unique-value!92 -> distinct-elems!84!val!6
-unique-value!93 -> distinct-elems!84!val!7
-unique-value!94 -> distinct-elems!84!val!8
-unique-value!95 -> distinct-elems!84!val!9
-unique-value!96 -> distinct-elems!84!val!10
-unique-value!97 -> distinct-elems!84!val!11
-unique-value!98 -> distinct-elems!84!val!12
-unique-value!99 -> distinct-elems!84!val!13
+unique-value!116 -> distinct-elems!114!val!0
+unique-value!117 -> distinct-elems!114!val!1
+unique-value!118 -> distinct-elems!114!val!2
+unique-value!119 -> distinct-elems!114!val!3
+unique-value!120 -> distinct-elems!114!val!4
+unique-value!121 -> distinct-elems!114!val!5
+unique-value!122 -> distinct-elems!114!val!6
+unique-value!123 -> distinct-elems!114!val!7
+unique-value!124 -> distinct-elems!114!val!8
+unique-value!125 -> distinct-elems!114!val!9
+unique-value!126 -> distinct-elems!114!val!10
+unique-value!127 -> distinct-elems!114!val!11
+unique-value!128 -> distinct-elems!114!val!12
+unique-value!129 -> distinct-elems!114!val!13
+unique-value!130 -> distinct-elems!114!val!14
+unique-value!131 -> distinct-elems!114!val!15
+unique-value!132 -> distinct-elems!114!val!16
+unique-value!133 -> distinct-elems!114!val!17
+unique-value!134 -> distinct-elems!114!val!18
+unique-value!135 -> distinct-elems!114!val!19
+unique-value!136 -> distinct-elems!114!val!20
+unique-value!137 -> distinct-elems!114!val!21
+unique-value!138 -> distinct-elems!114!val!22
+unique-value!139 -> distinct-elems!114!val!23
+unique-value!140 -> distinct-elems!114!val!24
+unique-value!141 -> distinct-elems!114!val!25
+unique-value!142 -> distinct-elems!114!val!26
+unique-value!143 -> distinct-elems!114!val!27
+unique-value!144 -> distinct-elems!114!val!28
+unique-value!145 -> distinct-elems!114!val!29
+unique-value!146 -> distinct-elems!114!val!30
+unique-value!147 -> distinct-elems!114!val!31
+unique-value!148 -> distinct-elems!114!val!32
+unique-value!149 -> distinct-elems!114!val!33
+unique-value!150 -> distinct-elems!114!val!34
+unique-value!151 -> distinct-elems!114!val!35
+unique-value!152 -> distinct-elems!114!val!36
+unique-value!153 -> distinct-elems!114!val!37
+unique-value!154 -> distinct-elems!114!val!38
+unique-value!155 -> distinct-elems!114!val!39
+unique-value!156 -> distinct-elems!114!val!40
+unique-value!157 -> distinct-elems!114!val!41
+unique-value!158 -> distinct-elems!114!val!42
+unique-value!159 -> distinct-elems!114!val!43
+unique-value!160 -> distinct-elems!114!val!44
+unique-value!161 -> distinct-elems!114!val!45
+unique-value!162 -> distinct-elems!114!val!46
+unique-value!163 -> distinct-elems!114!val!47
+unique-value!164 -> distinct-elems!114!val!48
+unique-value!165 -> distinct-elems!114!val!49
+unique-value!166 -> distinct-elems!114!val!50
+unique-value!167 -> distinct-elems!114!val!51
+unique-value!168 -> distinct-elems!114!val!52
+unique-value!169 -> distinct-elems!114!val!53
+unique-value!170 -> distinct-elems!114!val!54
+unique-value!171 -> distinct-elems!114!val!55
+unique-value!172 -> distinct-elems!114!val!56
+unique-value!173 -> distinct-elems!114!val!57
+unique-value!174 -> distinct-elems!114!val!58
+unique-value!175 -> distinct-elems!114!val!59
+unique-value!176 -> distinct-elems!114!val!60
+unique-value!177 -> distinct-elems!114!val!61
+unique-value!178 -> distinct-elems!114!val!62
 _System.array.Length -> {
   else -> 0
 }
@@ -1273,7 +1486,15 @@ $HeapSuccGhost -> {
   else -> false
 }
 $Is -> {
-  T@U!val!63 T@U!val!62 -> true
+  T@U!val!69 T@U!val!68 -> true
+  T@U!val!73 T@U!val!81 -> true
+  T@U!val!74 T@U!val!81 -> true
+  T@U!val!76 T@U!val!81 -> true
+  T@U!val!77 T@U!val!81 -> true
+  T@U!val!78 T@U!val!81 -> true
+  T@U!val!79 T@U!val!81 -> true
+  T@U!val!80 T@U!val!81 -> true
+  T@U!val!84 T@U!val!81 -> true
   else -> true
 }
 $IsA#_System.Tuple0 -> {
@@ -1283,7 +1504,15 @@ $IsA#_System.Tuple2 -> {
   else -> false
 }
 $IsAlloc -> {
-  else -> false
+  T@U!val!73 T@U!val!81 T@U!val!72 -> true
+  T@U!val!74 T@U!val!81 T@U!val!72 -> true
+  T@U!val!76 T@U!val!81 T@U!val!72 -> true
+  T@U!val!77 T@U!val!81 T@U!val!72 -> true
+  T@U!val!78 T@U!val!81 T@U!val!72 -> true
+  T@U!val!79 T@U!val!81 T@U!val!72 -> true
+  T@U!val!80 T@U!val!81 T@U!val!72 -> true
+  T@U!val!84 T@U!val!81 T@U!val!72 -> true
+  else -> true
 }
 $IsAllocBox -> {
   else -> false
@@ -1296,15 +1525,16 @@ $IsGhostField -> {
   else -> false
 }
 $IsGoodHeap -> {
-  T@U!val!58 -> true
-  T@U!val!65 -> true
+  T@U!val!64 -> true
+  T@U!val!72 -> true
   else -> true
 }
 $IsGoodMultiSet -> {
-  else -> false
+  T@U!val!85 -> true
+  else -> true
 }
 $IsHeapAnchor -> {
-  T@U!val!65 -> true
+  T@U!val!72 -> true
   else -> true
 }
 $LS -> {
@@ -1320,6 +1550,12 @@ Apply0 -> {
   else -> T@U!val!0
 }
 Apply1 -> {
+  else -> T@U!val!0
+}
+Apply3 -> {
+  else -> T@U!val!0
+}
+AsFuelBottom -> {
   else -> T@U!val!0
 }
 AtLayer -> {
@@ -1345,10 +1581,10 @@ char#ToInt -> {
   else -> 0
 }
 ControlFlow -> {
-  0 0 -> 63373
-  0 54326 -> (- 63460)
-  0 63373 -> 54326
-  else -> 63373
+  0 0 -> 123963
+  0 123963 -> 70422
+  0 70422 -> (- 124274)
+  else -> 123963
 }
 Ctor -> {
   T@T!val!0 -> 0
@@ -1365,7 +1601,9 @@ Ctor -> {
   T@T!val!19 -> 15
   T@T!val!2 -> 2
   T@T!val!20 -> 23
-  T@T!val!21 -> 25
+  T@T!val!21 -> 26
+  T@T!val!22 -> 16
+  T@T!val!23 -> 15
   T@T!val!3 -> 3
   T@T!val!4 -> 4
   T@T!val!5 -> 5
@@ -1373,11 +1611,11 @@ Ctor -> {
   T@T!val!7 -> 7
   T@T!val!8 -> 8
   T@T!val!9 -> 9
-  else -> 0
+  else -> 15
 }
 DatatypeCtorId -> {
-  T@U!val!63 -> T@U!val!40
-  else -> T@U!val!40
+  T@U!val!69 -> T@U!val!43
+  else -> T@U!val!43
 }
 DeclName -> {
   T@U!val!22 -> T@U!val!23
@@ -1386,65 +1624,71 @@ DeclName -> {
 DeclType -> {
   else -> T@U!val!0
 }
-distinct-aux-f!!85 -> {
-  T@U!val!0 -> distinct-elems!84!val!0
-  T@U!val!1 -> distinct-elems!84!val!1
-  T@U!val!10 -> distinct-elems!84!val!10
-  T@U!val!11 -> distinct-elems!84!val!11
-  T@U!val!12 -> distinct-elems!84!val!12
-  T@U!val!13 -> distinct-elems!84!val!13
-  T@U!val!14 -> distinct-elems!84!val!14
-  T@U!val!15 -> distinct-elems!84!val!15
-  T@U!val!16 -> distinct-elems!84!val!16
-  T@U!val!17 -> distinct-elems!84!val!17
-  T@U!val!18 -> distinct-elems!84!val!18
-  T@U!val!19 -> distinct-elems!84!val!19
-  T@U!val!2 -> distinct-elems!84!val!2
-  T@U!val!20 -> distinct-elems!84!val!20
-  T@U!val!21 -> distinct-elems!84!val!21
-  T@U!val!22 -> distinct-elems!84!val!22
-  T@U!val!23 -> distinct-elems!84!val!23
-  T@U!val!24 -> distinct-elems!84!val!24
-  T@U!val!25 -> distinct-elems!84!val!25
-  T@U!val!26 -> distinct-elems!84!val!26
-  T@U!val!27 -> distinct-elems!84!val!27
-  T@U!val!28 -> distinct-elems!84!val!28
-  T@U!val!29 -> distinct-elems!84!val!29
-  T@U!val!3 -> distinct-elems!84!val!3
-  T@U!val!30 -> distinct-elems!84!val!30
-  T@U!val!31 -> distinct-elems!84!val!31
-  T@U!val!32 -> distinct-elems!84!val!32
-  T@U!val!33 -> distinct-elems!84!val!33
-  T@U!val!34 -> distinct-elems!84!val!34
-  T@U!val!35 -> distinct-elems!84!val!35
-  T@U!val!36 -> distinct-elems!84!val!36
-  T@U!val!37 -> distinct-elems!84!val!37
-  T@U!val!38 -> distinct-elems!84!val!38
-  T@U!val!39 -> distinct-elems!84!val!39
-  T@U!val!4 -> distinct-elems!84!val!4
-  T@U!val!40 -> distinct-elems!84!val!40
-  T@U!val!41 -> distinct-elems!84!val!41
-  T@U!val!42 -> distinct-elems!84!val!42
-  T@U!val!43 -> distinct-elems!84!val!43
-  T@U!val!44 -> distinct-elems!84!val!44
-  T@U!val!45 -> distinct-elems!84!val!45
-  T@U!val!46 -> distinct-elems!84!val!46
-  T@U!val!47 -> distinct-elems!84!val!47
-  T@U!val!48 -> distinct-elems!84!val!48
-  T@U!val!49 -> distinct-elems!84!val!49
-  T@U!val!5 -> distinct-elems!84!val!5
-  T@U!val!50 -> distinct-elems!84!val!50
-  T@U!val!51 -> distinct-elems!84!val!51
-  T@U!val!52 -> distinct-elems!84!val!52
-  T@U!val!53 -> distinct-elems!84!val!53
-  T@U!val!54 -> distinct-elems!84!val!54
-  T@U!val!55 -> distinct-elems!84!val!55
-  T@U!val!56 -> distinct-elems!84!val!56
-  T@U!val!6 -> distinct-elems!84!val!6
-  T@U!val!7 -> distinct-elems!84!val!7
-  T@U!val!8 -> distinct-elems!84!val!8
-  T@U!val!9 -> distinct-elems!84!val!9
-  else -> distinct-elems!84!val!0
+distinct-aux-f!!115 -> {
+  T@U!val!0 -> distinct-elems!114!val!0
+  T@U!val!1 -> distinct-elems!114!val!1
+  T@U!val!10 -> distinct-elems!114!val!10
+  T@U!val!11 -> distinct-elems!114!val!11
+  T@U!val!12 -> distinct-elems!114!val!12
+  T@U!val!13 -> distinct-elems!114!val!13
+  T@U!val!14 -> distinct-elems!114!val!14
+  T@U!val!15 -> distinct-elems!114!val!15
+  T@U!val!16 -> distinct-elems!114!val!16
+  T@U!val!17 -> distinct-elems!114!val!17
+  T@U!val!18 -> distinct-elems!114!val!18
+  T@U!val!19 -> distinct-elems!114!val!19
+  T@U!val!2 -> distinct-elems!114!val!2
+  T@U!val!20 -> distinct-elems!114!val!20
+  T@U!val!21 -> distinct-elems!114!val!21
+  T@U!val!22 -> distinct-elems!114!val!22
+  T@U!val!23 -> distinct-elems!114!val!23
+  T@U!val!24 -> distinct-elems!114!val!24
+  T@U!val!25 -> distinct-elems!114!val!25
+  T@U!val!26 -> distinct-elems!114!val!26
+  T@U!val!27 -> distinct-elems!114!val!27
+  T@U!val!28 -> distinct-elems!114!val!28
+  T@U!val!29 -> distinct-elems!114!val!29
+  T@U!val!3 -> distinct-elems!114!val!3
+  T@U!val!30 -> distinct-elems!114!val!30
+  T@U!val!31 -> distinct-elems!114!val!31
+  T@U!val!32 -> distinct-elems!114!val!32
+  T@U!val!33 -> distinct-elems!114!val!33
+  T@U!val!34 -> distinct-elems!114!val!34
+  T@U!val!35 -> distinct-elems!114!val!35
+  T@U!val!36 -> distinct-elems!114!val!36
+  T@U!val!37 -> distinct-elems!114!val!37
+  T@U!val!38 -> distinct-elems!114!val!38
+  T@U!val!39 -> distinct-elems!114!val!39
+  T@U!val!4 -> distinct-elems!114!val!4
+  T@U!val!40 -> distinct-elems!114!val!40
+  T@U!val!41 -> distinct-elems!114!val!41
+  T@U!val!42 -> distinct-elems!114!val!42
+  T@U!val!43 -> distinct-elems!114!val!43
+  T@U!val!44 -> distinct-elems!114!val!44
+  T@U!val!45 -> distinct-elems!114!val!45
+  T@U!val!46 -> distinct-elems!114!val!46
+  T@U!val!47 -> distinct-elems!114!val!47
+  T@U!val!48 -> distinct-elems!114!val!48
+  T@U!val!49 -> distinct-elems!114!val!49
+  T@U!val!5 -> distinct-elems!114!val!5
+  T@U!val!50 -> distinct-elems!114!val!50
+  T@U!val!51 -> distinct-elems!114!val!51
+  T@U!val!52 -> distinct-elems!114!val!52
+  T@U!val!53 -> distinct-elems!114!val!53
+  T@U!val!54 -> distinct-elems!114!val!54
+  T@U!val!55 -> distinct-elems!114!val!55
+  T@U!val!56 -> distinct-elems!114!val!56
+  T@U!val!57 -> distinct-elems!114!val!57
+  T@U!val!58 -> distinct-elems!114!val!58
+  T@U!val!59 -> distinct-elems!114!val!59
+  T@U!val!6 -> distinct-elems!114!val!6
+  T@U!val!60 -> distinct-elems!114!val!60
+  T@U!val!61 -> distinct-elems!114!val!61
+  T@U!val!62 -> distinct-elems!114!val!62
+  T@U!val!7 -> distinct-elems!114!val!7
+  T@U!val!8 -> distinct-elems!114!val!8
+  T@U!val!9 -> distinct-elems!114!val!9
+  else -> distinct-elems!114!val!0
 }
 Div -> {
   else -> 0
@@ -1474,6 +1718,9 @@ Handle0 -> {
   else -> T@U!val!0
 }
 Handle1 -> {
+  else -> T@U!val!0
+}
+Handle3 -> {
   else -> T@U!val!0
 }
 IMap#Build -> {
@@ -1567,7 +1814,8 @@ Inv0_TMultiSet -> {
   else -> T@U!val!0
 }
 Inv0_TSeq -> {
-  else -> T@U!val!0
+  T@U!val!81 -> T@U!val!1
+  else -> T@U!val!1
 }
 Inv0_TSet -> {
   else -> T@U!val!0
@@ -1603,19 +1851,38 @@ ISet#UnionOne -> {
   else -> T@U!val!0
 }
 lambda#0 -> {
-  T@U!val!60 T@U!val!65 T@U!val!22 false -> T@U!val!66
-  else -> T@U!val!66
+  else -> T@U!val!0
+}
+lambda#1 -> {
+  else -> T@U!val!0
+}
+lambda#2 -> {
+  else -> T@U!val!0
+}
+lambda#3 -> {
+  T@U!val!66 T@U!val!72 T@U!val!22 false -> T@U!val!82
+  else -> T@U!val!82
 }
 Lit -> {
   false -> false
-  T@U!val!63 -> T@U!val!63
-  else -> T@U!val!63
+  T@U!val!69 -> T@U!val!69
+  else -> T@U!val!69
 }
 LitInt -> {
+  0 -> 0
   else -> 0
 }
 LitReal -> {
   else -> 0.0
+}
+M.__default.replaceRecursiveFunc -> {
+  else -> T@U!val!0
+}
+M.__default.replaceRecursiveFunc#canCall -> {
+  else -> false
+}
+M.__default.replaceRecursiveFunc#requires -> {
+  else -> false
 }
 Map#Build -> {
   else -> T@U!val!0
@@ -1663,15 +1930,18 @@ MapType0Store -> {
   else -> T@U!val!0
 }
 MapType0Type -> {
+  T@T!val!13 T@T!val!0 -> T@T!val!23
   T@T!val!16 T@T!val!15 -> T@T!val!19
   else -> T@T!val!19
 }
 MapType0TypeInv0 -> {
   T@T!val!19 -> T@T!val!16
+  T@T!val!23 -> T@T!val!13
   else -> T@T!val!16
 }
 MapType0TypeInv1 -> {
   T@T!val!19 -> T@T!val!15
+  T@T!val!23 -> T@T!val!0
   else -> T@T!val!15
 }
 MapType1Select -> {
@@ -1705,14 +1975,38 @@ MapType3Store -> {
   else -> T@U!val!0
 }
 MapType3Type -> {
+  else -> T@T!val!0
+}
+MapType3TypeInv0 -> {
+  else -> T@T!val!0
+}
+MapType3TypeInv1 -> {
+  else -> T@T!val!0
+}
+MapType3TypeInv2 -> {
+  else -> T@T!val!0
+}
+MapType3TypeInv3 -> {
+  else -> T@T!val!0
+}
+MapType3TypeInv4 -> {
+  else -> T@T!val!0
+}
+MapType4Select -> {
+  else -> T@U!val!0
+}
+MapType4Store -> {
+  else -> T@U!val!0
+}
+MapType4Type -> {
   T@T!val!16 T@T!val!2 -> T@T!val!21
   else -> T@T!val!21
 }
-MapType3TypeInv0 -> {
+MapType4TypeInv0 -> {
   T@T!val!21 -> T@T!val!16
   else -> T@T!val!16
 }
-MapType3TypeInv1 -> {
+MapType4TypeInv1 -> {
   T@T!val!21 -> T@T!val!2
   else -> T@T!val!2
 }
@@ -1753,13 +2047,15 @@ MultiSet#Disjoint -> {
   else -> false
 }
 MultiSet#Empty -> {
-  else -> T@U!val!0
+  T@T!val!13 -> T@U!val!85
+  else -> T@U!val!85
 }
 MultiSet#Equal -> {
   else -> false
 }
 MultiSet#FromSeq -> {
-  else -> T@U!val!0
+  T@U!val!84 -> T@U!val!85
+  else -> T@U!val!85
 }
 MultiSet#FromSet -> {
   else -> T@U!val!0
@@ -1812,6 +2108,9 @@ Reads0 -> {
 Reads1 -> {
   else -> T@U!val!0
 }
+Reads3 -> {
+  else -> T@U!val!0
+}
 real_2_U -> {
   else -> T@U!val!0
 }
@@ -1825,6 +2124,9 @@ Requires0 -> {
   else -> false
 }
 Requires1 -> {
+  else -> false
+}
+Requires3 -> {
   else -> false
 }
 rmode_2_U -> {
@@ -1852,7 +2154,8 @@ Seq#Drop -> {
   else -> T@U!val!0
 }
 Seq#Empty -> {
-  else -> T@U!val!0
+  T@T!val!13 -> T@U!val!84
+  else -> T@U!val!84
 }
 Seq#Equal -> {
   else -> false
@@ -1864,7 +2167,10 @@ Seq#Index -> {
   else -> T@U!val!0
 }
 Seq#Length -> {
-  else -> 0
+  T@U!val!73 -> 1
+  T@U!val!74 -> 1
+  T@U!val!84 -> 0
+  else -> 1
 }
 Seq#Rank -> {
   else -> 0
@@ -1882,10 +2188,12 @@ Seq#Update -> {
   else -> T@U!val!0
 }
 SeqType -> {
-  else -> T@T!val!0
+  T@T!val!13 -> T@T!val!22
+  else -> T@T!val!22
 }
 SeqTypeInv0 -> {
-  else -> T@T!val!0
+  T@T!val!22 -> T@T!val!13
+  else -> T@T!val!13
 }
 Set#Card -> {
   else -> 0
@@ -1932,20 +2240,21 @@ Tag -> {
   T@U!val!2 -> T@U!val!7
   T@U!val!3 -> T@U!val!8
   T@U!val!4 -> T@U!val!9
-  T@U!val!57 -> T@U!val!26
-  T@U!val!59 -> T@U!val!24
-  T@U!val!61 -> T@U!val!27
-  T@U!val!62 -> T@U!val!41
-  T@U!val!64 -> T@U!val!44
+  T@U!val!63 -> T@U!val!26
+  T@U!val!65 -> T@U!val!24
+  T@U!val!67 -> T@U!val!27
+  T@U!val!68 -> T@U!val!44
+  T@U!val!70 -> T@U!val!47
+  T@U!val!81 -> T@U!val!13
   else -> T@U!val!5
 }
 TagFamily -> {
-  T@U!val!57 -> T@U!val!46
-  T@U!val!59 -> T@U!val!45
-  T@U!val!61 -> T@U!val!46
-  T@U!val!62 -> T@U!val!55
-  T@U!val!64 -> T@U!val!56
-  else -> T@U!val!46
+  T@U!val!63 -> T@U!val!49
+  T@U!val!65 -> T@U!val!48
+  T@U!val!67 -> T@U!val!49
+  T@U!val!68 -> T@U!val!61
+  T@U!val!70 -> T@U!val!62
+  else -> T@U!val!49
 }
 TBitvector -> {
   else -> T@U!val!0
@@ -1965,6 +2274,21 @@ Tclass._System.___hFunc1_0 -> {
 Tclass._System.___hFunc1_1 -> {
   else -> T@U!val!0
 }
+Tclass._System.___hFunc3 -> {
+  else -> T@U!val!0
+}
+Tclass._System.___hFunc3_0 -> {
+  else -> T@U!val!0
+}
+Tclass._System.___hFunc3_1 -> {
+  else -> T@U!val!0
+}
+Tclass._System.___hFunc3_2 -> {
+  else -> T@U!val!0
+}
+Tclass._System.___hFunc3_3 -> {
+  else -> T@U!val!0
+}
 Tclass._System.___hPartialFunc0 -> {
   else -> T@U!val!0
 }
@@ -1980,6 +2304,21 @@ Tclass._System.___hPartialFunc1_0 -> {
 Tclass._System.___hPartialFunc1_1 -> {
   else -> T@U!val!0
 }
+Tclass._System.___hPartialFunc3 -> {
+  else -> T@U!val!0
+}
+Tclass._System.___hPartialFunc3_0 -> {
+  else -> T@U!val!0
+}
+Tclass._System.___hPartialFunc3_1 -> {
+  else -> T@U!val!0
+}
+Tclass._System.___hPartialFunc3_2 -> {
+  else -> T@U!val!0
+}
+Tclass._System.___hPartialFunc3_3 -> {
+  else -> T@U!val!0
+}
 Tclass._System.___hTotalFunc0 -> {
   else -> T@U!val!0
 }
@@ -1993,6 +2332,21 @@ Tclass._System.___hTotalFunc1_0 -> {
   else -> T@U!val!0
 }
 Tclass._System.___hTotalFunc1_1 -> {
+  else -> T@U!val!0
+}
+Tclass._System.___hTotalFunc3 -> {
+  else -> T@U!val!0
+}
+Tclass._System.___hTotalFunc3_0 -> {
+  else -> T@U!val!0
+}
+Tclass._System.___hTotalFunc3_1 -> {
+  else -> T@U!val!0
+}
+Tclass._System.___hTotalFunc3_2 -> {
+  else -> T@U!val!0
+}
+Tclass._System.___hTotalFunc3_3 -> {
   else -> T@U!val!0
 }
 Tclass._System.array -> {
@@ -2034,7 +2388,8 @@ TMultiSet -> {
   else -> T@U!val!0
 }
 TSeq -> {
-  else -> T@U!val!0
+  T@U!val!1 -> T@U!val!81
+  else -> T@U!val!81
 }
 TSet -> {
   else -> T@U!val!0
@@ -2072,18 +2427,18 @@ type -> {
   T@U!val!34 -> T@T!val!7
   T@U!val!35 -> T@T!val!7
   T@U!val!36 -> T@T!val!7
-  T@U!val!37 -> T@T!val!11
+  T@U!val!37 -> T@T!val!7
   T@U!val!38 -> T@T!val!7
-  T@U!val!39 -> T@T!val!8
+  T@U!val!39 -> T@T!val!7
   T@U!val!4 -> T@T!val!6
   T@U!val!40 -> T@T!val!11
   T@U!val!41 -> T@T!val!7
   T@U!val!42 -> T@T!val!8
-  T@U!val!43 -> T@T!val!8
+  T@U!val!43 -> T@T!val!11
   T@U!val!44 -> T@T!val!7
-  T@U!val!45 -> T@T!val!12
-  T@U!val!46 -> T@T!val!12
-  T@U!val!47 -> T@T!val!12
+  T@U!val!45 -> T@T!val!8
+  T@U!val!46 -> T@T!val!8
+  T@U!val!47 -> T@T!val!7
   T@U!val!48 -> T@T!val!12
   T@U!val!49 -> T@T!val!12
   T@U!val!5 -> T@T!val!7
@@ -2094,19 +2449,37 @@ type -> {
   T@U!val!54 -> T@T!val!12
   T@U!val!55 -> T@T!val!12
   T@U!val!56 -> T@T!val!12
-  T@U!val!57 -> T@T!val!6
-  T@U!val!58 -> T@T!val!19
-  T@U!val!59 -> T@T!val!6
+  T@U!val!57 -> T@T!val!12
+  T@U!val!58 -> T@T!val!12
+  T@U!val!59 -> T@T!val!12
   T@U!val!6 -> T@T!val!7
-  T@U!val!60 -> T@T!val!16
-  T@U!val!61 -> T@T!val!6
-  T@U!val!62 -> T@T!val!6
-  T@U!val!63 -> T@T!val!17
-  T@U!val!64 -> T@T!val!6
-  T@U!val!65 -> T@T!val!19
-  T@U!val!66 -> T@T!val!21
+  T@U!val!60 -> T@T!val!12
+  T@U!val!61 -> T@T!val!12
+  T@U!val!62 -> T@T!val!12
+  T@U!val!63 -> T@T!val!6
+  T@U!val!64 -> T@T!val!19
+  T@U!val!65 -> T@T!val!6
+  T@U!val!66 -> T@T!val!16
+  T@U!val!67 -> T@T!val!6
+  T@U!val!68 -> T@T!val!6
+  T@U!val!69 -> T@T!val!17
   T@U!val!7 -> T@T!val!7
+  T@U!val!70 -> T@T!val!6
+  T@U!val!71 -> T@T!val!18
+  T@U!val!72 -> T@T!val!19
+  T@U!val!73 -> T@T!val!22
+  T@U!val!74 -> T@T!val!22
+  T@U!val!75 -> T@T!val!22
+  T@U!val!76 -> T@T!val!22
+  T@U!val!77 -> T@T!val!22
+  T@U!val!78 -> T@T!val!22
+  T@U!val!79 -> T@T!val!22
   T@U!val!8 -> T@T!val!7
+  T@U!val!80 -> T@T!val!22
+  T@U!val!81 -> T@T!val!6
+  T@U!val!82 -> T@T!val!21
+  T@U!val!84 -> T@T!val!22
+  T@U!val!85 -> T@T!val!23
   T@U!val!9 -> T@T!val!7
   else -> T@T!val!7
 }
@@ -2147,14 +2520,26 @@ UOrdering3 -> {
 *** STATE <initial>
   $_Frame -> 
   $_reverifyPost -> 
-  $Heap -> T@U!val!65
+  $Heap -> T@U!val!72
+  $rhs##1_0 -> T@U!val!77
+  $rhs##2_0 -> T@U!val!80
   $Tick -> 
-  a#0 -> 11
-  b#0 -> 5
-  c#0 -> 
-  defass#c#0 -> 
+  defass#newString#0 -> false
+  first#2_0 -> T@U!val!78
+  inner#2_0 -> T@U!val!79
+  newString#0 -> T@U!val!75
+  other##1_0 -> 
+  other##2_0 -> 
+  other#0 -> T@U!val!74
+  pattern##1_0 -> 
+  pattern##2_0 -> 
+  pattern#0 -> T@U!val!84
+  prefixedInner#1_0 -> T@U!val!76
+  remainingString##1_0 -> 
+  remainingString##2_0 -> 
+  remainingString#0 -> T@U!val!73
 *** END_STATE
-*** STATE /workspaces/dafny/string_project/str_recurse.dfy(5,2): initial state
-  $_Frame -> T@U!val!66
+*** STATE /workspaces/dafny/string_project/str_recurse.dfy(35,2): initial state
+  $_Frame -> T@U!val!82
 *** END_STATE
 *** END_MODEL
